Finish Encryption tests

fstar/new/Test_Equality.ml
@@ -1,0 +1,1 @@
+let test_equality x y = x = y
