fstar/new/NetworkTypes.fst
@@ -1,6 +1,7 @@
 module NetworkTypes
 
 open Lib.IntTypes
+open Lib.ByteSequence
 open Parser
 open Crypto.Builtins
 
@@ -468,3 +469,684 @@ type ratchet_tree_nt = blseq (option_nt node_nt) (ps_option ps_node) ({min=1; ma
 
 val ps_ratchet_tree: parser_serializer ratchet_tree_nt
 let ps_ratchet_tree = ps_seq _ (ps_option ps_node)
+
+type psk_type_nt =
+  | PSKT_reserved: psk_type_nt
+  | PSKT_external: psk_type_nt
+  | PSKT_reinit: psk_type_nt
+  | PSKT_branch: psk_type_nt
+  | PSKT_unknown: n:nat{4 <= n /\ n < 256} -> psk_type_nt
+
+val ps_psk_type: parser_serializer psk_type_nt
+let ps_psk_type =
+  isomorphism psk_type_nt ps_u8
+    (fun x -> match v x with
+      | 0 -> PSKT_reserved
+      | 1 -> PSKT_external
+      | 2 -> PSKT_reinit
+      | 3 -> PSKT_branch
+      | vx -> PSKT_unknown vx
+    )
+    (fun x -> match x with
+      | PSKT_reserved -> u8 0
+      | PSKT_external -> u8 1
+      | PSKT_reinit -> u8 2
+      | PSKT_branch -> u8 3
+      | PSKT_unknown vx -> u8 vx
+    )
+
+val get_psk_type: psk_type_nt -> Type0
+let get_psk_type psk_type =
+  match psk_type with
+  | PSKT_external -> blbytes ({min=0; max=255})
+  | PSKT_reinit -> (x:blbytes ({min=0; max=255})) & uint64
+  | PSKT_branch -> (x:blbytes ({min=0; max=255})) & uint64
+  | _ -> unit
+
+noeq type pre_shared_key_id_nt =
+  | PSKI_reserved: psk_nonce:blbytes ({min=0; max=255}) -> pre_shared_key_id_nt
+  | PSKI_external: psk_id:blbytes ({min=0; max=255}) -> psk_nonce:blbytes ({min=0; max=255}) -> pre_shared_key_id_nt
+  | PSKI_reinit: psk_group_id:blbytes ({min=0; max=255}) -> psk_epoch:uint64 -> psk_nonce:blbytes ({min=0; max=255}) -> pre_shared_key_id_nt
+  | PSKI_branch: psk_group_id:blbytes ({min=0; max=255}) -> psk_epoch:uint64 -> psk_nonce:blbytes ({min=0; max=255}) -> pre_shared_key_id_nt
+  | PSKI_unknown: n:nat{4 <= n /\ n < 256} -> psk_nonce:blbytes ({min=0; max=255}) -> pre_shared_key_id_nt
+
+val ps_pre_shared_key_id: parser_serializer pre_shared_key_id_nt
+let ps_pre_shared_key_id =
+  isomorphism pre_shared_key_id_nt
+    (
+      _ <-- bind #_ #get_psk_type
+      ps_psk_type (fun psk_type ->
+        match psk_type with
+        | PSKT_reserved -> ps_unit
+        | PSKT_external -> (
+          ps_bytes ({min=0; max=255})
+        )
+        | PSKT_reinit -> (
+          _ <-- ps_bytes ({min=0; max=255});
+          ps_u64
+        )
+        | PSKT_branch -> (
+          _ <-- ps_bytes ({min=0; max=255});
+          ps_u64
+        )
+        | PSKT_unknown _ -> ps_unit
+      );
+      ps_bytes _
+    )
+    (fun (|(|psk_type, psk_value|), psk_nonce|) ->
+      match psk_type with
+      | PSKT_reserved -> PSKI_reserved psk_nonce
+      | PSKT_external ->
+        let psk_id: (blbytes ({min=0; max=255})) = psk_value in
+        PSKI_external psk_id psk_nonce
+      | PSKT_reinit ->
+        let (|psk_group_id, psk_epoch|) = (psk_value <: get_psk_type PSKT_reinit) in
+        PSKI_reinit psk_group_id psk_epoch psk_nonce
+      | PSKT_branch ->
+        let (|psk_group_id, psk_epoch|) = (psk_value <: get_psk_type PSKT_branch) in
+        PSKI_branch psk_group_id psk_epoch psk_nonce
+      | PSKT_unknown vx -> PSKI_unknown vx psk_nonce
+    )
+    (fun x ->
+      match x with
+      | PSKI_reserved psk_nonce -> (|(|PSKT_reserved, ()|), psk_nonce|)
+      | PSKI_external psk_id psk_nonce -> (|(|PSKT_external, psk_id|), psk_nonce|)
+      | PSKI_reinit psk_group_id psk_epoch psk_nonce -> (|(|PSKT_reinit, (|psk_group_id, psk_epoch|)|), psk_nonce|)
+      | PSKI_branch psk_group_id psk_epoch psk_nonce -> (|(|PSKT_branch, (|psk_group_id, psk_epoch|)|), psk_nonce|)
+      | PSKI_unknown vx psk_nonce -> (|(|PSKT_unknown vx, ()|), psk_nonce|)
+    )
+
+noeq type pre_shared_keys_nt = {
+  pskn_psks: blseq pre_shared_key_id_nt ps_pre_shared_key_id ({min=0; max=(pow2 16)-1});
+}
+
+val ps_pre_shared_keys: parser_serializer pre_shared_keys_nt
+let ps_pre_shared_keys =
+  isomorphism pre_shared_keys_nt
+    (ps_seq _ ps_pre_shared_key_id)
+    (fun psks -> {pskn_psks = psks})
+    (fun x -> x.pskn_psks)
+
+(*** Proposals ***)
+
+noeq type add_nt = {
+  an_key_package: key_package_nt;
+}
+
+val ps_add: parser_serializer add_nt
+let ps_add =
+  isomorphism add_nt ps_key_package
+    (fun key_package -> ({ an_key_package = key_package }))
+    (fun x -> x.an_key_package)
+
+noeq type update_nt = {
+  un_key_package: key_package_nt;
+}
+
+val ps_update: parser_serializer update_nt
+let ps_update =
+  isomorphism update_nt ps_key_package
+    (fun key_package -> ({ un_key_package = key_package }))
+    (fun x -> x.un_key_package)
+
+noeq type remove_nt = {
+  rn_removed: uint32;
+}
+
+val ps_remove: parser_serializer remove_nt
+let ps_remove =
+  isomorphism remove_nt ps_u32
+    (fun removed -> ({ rn_removed = removed }))
+    (fun x -> x.rn_removed)
+
+noeq type pre_shared_key_nt = {
+  pskn_psk: pre_shared_key_id_nt;
+}
+
+val ps_pre_shared_key: parser_serializer pre_shared_key_nt
+let ps_pre_shared_key =
+  isomorphism pre_shared_key_nt ps_pre_shared_key_id
+    (fun psk -> {pskn_psk = psk})
+    (fun x -> x.pskn_psk)
+
+noeq type reinit_nt = {
+  rin_group_id: blbytes ({min=0; max=255});
+  rin_version: protocol_version_nt;
+  rin_cipher_suite: cipher_suite_nt;
+  rin_extensions: blseq extension_nt ps_extension ({min=0; max=(pow2 32)-1})
+}
+
+val ps_reinit: parser_serializer reinit_nt
+let ps_reinit =
+  isomorphism reinit_nt
+    (
+      _ <-- ps_bytes _;
+      _ <-- ps_protocol_version;
+      _ <-- ps_cipher_suite;
+      ps_seq _ ps_extension
+    )
+    (fun (|group_id, (|version, (|cipher_suite, extensions|)|)|) -> ({
+      rin_group_id = group_id;
+      rin_version = version;
+      rin_cipher_suite = cipher_suite;
+      rin_extensions = extensions;
+    }))
+    (fun x -> (|x.rin_group_id, (|x.rin_version, (|x.rin_cipher_suite, x.rin_extensions|)|)|))
+
+noeq type external_init_nt = {
+  ein_kem_output: blbytes ({min=0; max=(pow2 16)-1})
+}
+
+val ps_external_init: parser_serializer external_init_nt
+let ps_external_init =
+  isomorphism external_init_nt
+    (ps_bytes _)
+    (fun kem_output -> {ein_kem_output = kem_output})
+    (fun x -> x.ein_kem_output)
+
+noeq type message_range_nt = {
+  mrn_sender: uint32;
+  mrn_first_generation: uint32;
+  mrn_last_generation: uint32;
+}
+
+val ps_message_range: parser_serializer message_range_nt
+let ps_message_range =
+  isomorphism message_range_nt
+    (
+      _ <-- ps_u32;
+      _ <-- ps_u32;
+      ps_u32
+    )
+    (fun (|sender, (|first_generation, last_generation|)|) -> ({
+      mrn_sender = sender;
+      mrn_first_generation = first_generation;
+      mrn_last_generation = last_generation;
+    }))
+    (fun x -> (|x.mrn_sender, (|x.mrn_first_generation, x.mrn_last_generation|)|))
+
+noeq type app_ack_nt = {
+  aan_received_ranges: blseq message_range_nt ps_message_range ({min=0; max=(pow2 32)-1})
+}
+
+val ps_app_ack: parser_serializer app_ack_nt
+let ps_app_ack =
+  isomorphism app_ack_nt
+    (ps_seq _ ps_message_range)
+    (fun received_ranges -> {aan_received_ranges = received_ranges})
+    (fun x -> x.aan_received_ranges)
+
+type proposal_type_nt =
+  | PT_reserved: proposal_type_nt
+  | PT_add: proposal_type_nt
+  | PT_update: proposal_type_nt
+  | PT_remove: proposal_type_nt
+  | PT_psk: proposal_type_nt
+  | PT_reinit: proposal_type_nt
+  | PT_external_init: proposal_type_nt
+  | PT_app_ack: proposal_type_nt
+  | PT_unknown: n:nat{8 <= n /\ n < 256} -> proposal_type_nt
+
+val ps_proposal_type: parser_serializer proposal_type_nt
+let ps_proposal_type =
+  isomorphism proposal_type_nt ps_u8
+    (fun x -> match v x with
+      | 0 -> PT_reserved
+      | 1 -> PT_add
+      | 2 -> PT_update
+      | 3 -> PT_remove
+      | 4 -> PT_psk
+      | 5 -> PT_reinit
+      | 6 -> PT_external_init
+      | 7 -> PT_app_ack
+      | vx -> PT_unknown vx
+    )
+    (fun x -> match x with
+      | PT_reserved -> u8 0
+      | PT_add -> u8 1
+      | PT_update -> u8 2
+      | PT_remove -> u8 3
+      | PT_psk -> u8 4
+      | PT_reinit -> u8 5
+      | PT_external_init -> u8 6
+      | PT_app_ack -> u8 7
+      | PT_unknown vx -> u8 vx
+    )
+
+val get_proposal_type: proposal_type_nt -> Type0
+let get_proposal_type proposal_type =
+  match proposal_type with
+  | PT_reserved -> unit
+  | PT_add -> add_nt
+  | PT_update -> update_nt
+  | PT_remove -> remove_nt
+  | PT_psk -> pre_shared_key_nt
+  | PT_reinit -> reinit_nt
+  | PT_external_init -> external_init_nt
+  | PT_app_ack -> app_ack_nt
+  | PT_unknown vx -> unit
+
+noeq type proposal_nt =
+  | P_reserved: proposal_nt
+  | P_add: add_nt -> proposal_nt
+  | P_update: update_nt -> proposal_nt
+  | P_remove: remove_nt -> proposal_nt
+  | P_psk: pre_shared_key_nt -> proposal_nt
+  | P_reinit: reinit_nt -> proposal_nt
+  | P_external_init: external_init_nt -> proposal_nt
+  | P_app_ack: app_ack_nt -> proposal_nt
+  | P_unknown: n:nat{8 <= n /\ n < 256} -> proposal_nt
+
+val ps_proposal: parser_serializer proposal_nt
+let ps_proposal =
+  isomorphism proposal_nt
+    (
+      bind #_ #get_proposal_type
+      ps_proposal_type (fun proposal_type ->
+        match proposal_type with
+        | PT_reserved -> ps_unit
+        | PT_add -> ps_add
+        | PT_update -> ps_update
+        | PT_remove -> ps_remove
+        | PT_psk -> ps_pre_shared_key
+        | PT_reinit -> ps_reinit
+        | PT_external_init -> ps_external_init
+        | PT_app_ack -> ps_app_ack
+        | PT_unknown vx -> ps_unit
+      )
+    )
+    (fun (|proposal_type, proposal_value|) ->
+      match proposal_type with
+      | PT_reserved -> P_reserved
+      | PT_add -> P_add proposal_value
+      | PT_update -> P_update proposal_value
+      | PT_remove -> P_remove proposal_value
+      | PT_psk -> P_psk proposal_value
+      | PT_reinit -> P_reinit proposal_value
+      | PT_external_init -> P_external_init proposal_value
+      | PT_app_ack -> P_app_ack proposal_value
+      | PT_unknown vx -> P_unknown vx
+    )
+    (fun proposal -> match proposal with
+      | P_reserved -> (|PT_reserved, ()|)
+      | P_add x -> (|PT_add, x|)
+      | P_update x -> (|PT_update, x|)
+      | P_remove x -> (|PT_remove, x|)
+      | P_psk x -> (|PT_psk, x|)
+      | P_reinit x -> (|PT_reinit, x|)
+      | P_external_init x -> (|PT_external_init, x|)
+      | P_app_ack x -> (|PT_app_ack, x|)
+      | P_unknown vx -> (|PT_unknown vx, ()|)
+    )
+
+(*** Message framing ***)
+
+type proposal_or_ref_type_nt =
+  | PORT_reserved: proposal_or_ref_type_nt
+  | PORT_proposal: proposal_or_ref_type_nt
+  | PORT_reference: proposal_or_ref_type_nt
+  | PORT_unknown: n:nat{3 <= n /\ n < 256} -> proposal_or_ref_type_nt
+
+val ps_proposal_or_ref_type: parser_serializer proposal_or_ref_type_nt
+let ps_proposal_or_ref_type =
+  isomorphism proposal_or_ref_type_nt ps_u8
+    (fun x -> match v x with
+      | 0 -> PORT_reserved
+      | 1 -> PORT_proposal
+      | 2 -> PORT_reference
+      | vx -> PORT_unknown vx
+    )
+    (fun x -> match x with
+      | PORT_reserved -> u8 0
+      | PORT_proposal -> u8 1
+      | PORT_reference -> u8 2
+      | PORT_unknown vx -> u8 vx
+    )
+
+val get_proposal_or_ref_type: proposal_or_ref_type_nt -> Type0
+let get_proposal_or_ref_type proposal_or_ref_type =
+  match proposal_or_ref_type with
+  | PORT_proposal -> proposal_nt
+  | PORT_reference -> blbytes ({min=0; max=255})
+  | _ -> unit
+
+noeq type proposal_or_ref_nt =
+  | POR_reserved: proposal_or_ref_nt
+  | POR_proposal: proposal_nt -> proposal_or_ref_nt
+  | POR_reference: blbytes ({min=0; max=255}) -> proposal_or_ref_nt
+  | POR_unknown: n:nat{3 <= n /\ n < 256} -> proposal_or_ref_nt
+
+val ps_proposal_or_ref: parser_serializer proposal_or_ref_nt
+let ps_proposal_or_ref =
+  isomorphism proposal_or_ref_nt
+    (
+      bind #_ #get_proposal_or_ref_type
+      ps_proposal_or_ref_type (fun proposal_or_ref_type ->
+        match proposal_or_ref_type with
+        | PORT_proposal -> ps_proposal
+        | PORT_reference -> ps_bytes ({min=0; max=255})
+        | _ -> ps_unit
+      )
+    )
+    (fun (|proposal_or_ref_type, proposal_or_ref_value|) ->
+      match proposal_or_ref_type with
+      | PORT_reserved -> POR_reserved
+      | PORT_proposal -> POR_proposal proposal_or_ref_value
+      | PORT_reference -> POR_reference proposal_or_ref_value
+      | PORT_unknown vx -> POR_unknown vx
+    )
+    (fun x -> match x with
+      | POR_reserved -> (|PORT_reserved, ()|)
+      | POR_proposal x -> (|PORT_proposal, x|)
+      | POR_reference x -> (|PORT_reference, x|)
+      | POR_unknown vx -> (|PORT_unknown vx, ()|)
+    )
+
+noeq type commit_nt = {
+  cn_proposals: blseq proposal_or_ref_nt ps_proposal_or_ref ({min=0; max=(pow2 32)-1});
+  cn_path: option_nt (update_path_nt);
+}
+
+val ps_commit: parser_serializer commit_nt
+let ps_commit =
+  isomorphism commit_nt
+    (
+      _ <-- ps_seq _ ps_proposal_or_ref;
+      ps_option ps_update_path
+    )
+    (fun (|proposals, path|) -> ({
+      cn_proposals = proposals;
+      cn_path = path;
+    }))
+    (fun x -> (|x.cn_proposals, x.cn_path|))
+
+type sender_type_nt =
+  | ST_reserved: sender_type_nt
+  | ST_member: sender_type_nt
+  | ST_preconfigured: sender_type_nt
+  | ST_new_member: sender_type_nt
+  | ST_unknown: n:nat{4 <= n /\ n < 256} -> sender_type_nt
+
+val ps_sender_type: parser_serializer sender_type_nt
+let ps_sender_type =
+  isomorphism sender_type_nt ps_u8
+    (fun x -> match v x with
+      | 0 -> ST_reserved
+      | 1 -> ST_member
+      | 2 -> ST_preconfigured
+      | 3 -> ST_new_member
+      | vx -> ST_unknown vx
+    )
+    (fun x -> match x with
+      | ST_reserved -> u8 0
+      | ST_member -> u8 1
+      | ST_preconfigured -> u8 2
+      | ST_new_member -> u8 3
+      | ST_unknown vx -> u8 vx
+    )
+
+type sender_nt = {
+  sn_sender_type: sender_type_nt;
+  sn_sender: uint32;
+}
+
+val ps_sender: parser_serializer sender_nt
+let ps_sender =
+  isomorphism sender_nt
+    (
+      _ <-- ps_sender_type;
+      ps_u32
+    )
+    (fun (|sender_type, sender|) -> ({
+      sn_sender_type = sender_type;
+      sn_sender = sender;
+    }))
+    (fun x -> (|x.sn_sender_type, x.sn_sender|))
+
+type mac_nt = {
+  mn_mac_value: blbytes ({min=0; max=255});
+}
+
+val ps_mac: parser_serializer mac_nt
+let ps_mac =
+  isomorphism mac_nt (ps_bytes _)
+    (fun mac_value -> {mn_mac_value = mac_value})
+    (fun x -> x.mn_mac_value)
+
+//CT_reserved and CT_unknown already exist in credential_type_nt...
+type content_type_nt =
+  | CT_reserved2: content_type_nt
+  | CT_application: content_type_nt
+  | CT_proposal: content_type_nt
+  | CT_commit: content_type_nt
+  | CT_unknown2: n:nat{4 <= n /\ n < 256} -> content_type_nt
+
+val ps_content_type: parser_serializer content_type_nt
+let ps_content_type =
+  isomorphism content_type_nt ps_u8
+    (fun x -> match v x with
+      | 0 -> CT_reserved2
+      | 1 -> CT_application
+      | 2 -> CT_proposal
+      | 3 -> CT_commit
+      | vx -> CT_unknown2 vx
+    )
+    (fun x -> match x with
+      | CT_reserved2 -> u8 0
+      | CT_application -> u8 1
+      | CT_proposal -> u8 2
+      | CT_commit -> u8 3
+      | CT_unknown2 vx -> u8 vx
+    )
+
+val get_content_type: content_type_nt -> Type0
+let get_content_type content_type =
+  match content_type with
+  | CT_application -> blbytes ({min=0; max=(pow2 32)-1})
+  | CT_proposal -> proposal_nt
+  | CT_commit -> commit_nt
+  | _ -> unit
+
+noeq type mls_content_nt =
+  | MC_reserved: mls_content_nt
+  | MC_application: blbytes ({min=0; max=(pow2 32)-1}) -> mls_content_nt
+  | MC_proposal: proposal_nt -> mls_content_nt
+  | MC_commit: commit_nt -> mls_content_nt
+  | MC_unknown: n:nat{4 <= n /\ n < 256} -> mls_content_nt
+
+val ps_mls_content: parser_serializer mls_content_nt
+let ps_mls_content =
+  isomorphism mls_content_nt
+    (
+      bind #_ #get_content_type
+      ps_content_type (fun content_type ->
+        match content_type with
+        | CT_application -> ps_bytes ({min=0; max=(pow2 32)-1})
+        | CT_proposal -> ps_proposal
+        | CT_commit -> ps_commit
+        | _ -> ps_unit
+      )
+    )
+      (fun (|content_type, content_value|) ->
+        match content_type with
+        | CT_reserved2 -> MC_reserved
+        | CT_application -> MC_application content_value
+        | CT_proposal -> MC_proposal content_value
+        | CT_commit -> MC_commit content_value
+        | CT_unknown2 vx -> MC_unknown vx
+      )
+      (fun x ->
+        match x with
+        | MC_reserved -> (|CT_reserved2, ()|)
+        | MC_application x -> (|CT_application, x|)
+        | MC_proposal x -> (|CT_proposal, x|)
+        | MC_commit x -> (|CT_commit, x|)
+        | MC_unknown vx -> (|CT_unknown2 vx, ()|)
+      )
+
+noeq type mls_plaintext_nt = {
+  mpn_group_id: blbytes ({min=0; max=255});
+  mpn_epoch: uint64;
+  mpn_sender: sender_nt;
+  mpn_authenticated_data: blbytes ({min=0; max=(pow2 32)-1});
+  mpn_content: mls_content_nt;
+  mpn_signature: blbytes ({min=0; max=(pow2 16)-1});
+  mpn_confirmation_tag: option_nt mac_nt;
+  mpn_membership_tag: option_nt mac_nt;
+}
+
+#push-options "--ifuel 6"
+val ps_mls_plaintext: parser_serializer mls_plaintext_nt
+let ps_mls_plaintext =
+  isomorphism mls_plaintext_nt
+    (
+      _ <-- ps_bytes _;
+      _ <-- ps_u64;
+      _ <-- ps_sender;
+      _ <-- ps_bytes _;
+      _ <-- ps_mls_content;
+      _ <-- ps_bytes _;
+      _ <-- ps_option ps_mac;
+      ps_option ps_mac
+    )
+    (fun (|group_id, (|epoch, (|sender, (|authenticated_data, (|content, (|signature, (|confirmation_tag, membership_tag|)|)|)|)|)|)|) -> ({
+      mpn_group_id = group_id;
+      mpn_epoch = epoch;
+      mpn_sender = sender;
+      mpn_authenticated_data = authenticated_data;
+      mpn_content = content;
+      mpn_signature = signature;
+      mpn_confirmation_tag = confirmation_tag;
+      mpn_membership_tag = membership_tag;
+    }))
+    (fun x -> (|x.mpn_group_id, (|x.mpn_epoch, (|x.mpn_sender, (|x.mpn_authenticated_data, (|x.mpn_content, (|x.mpn_signature, (|x.mpn_confirmation_tag, x.mpn_membership_tag|)|)|)|)|)|)|))
+#pop-options
+
+noeq type mls_ciphertext_nt = {
+  mcn_group_id: blbytes ({min=0; max=255});
+  mcn_epoch: uint64;
+  mcn_content_type: content_type_nt;
+  mcn_authenticated_data: blbytes ({min=0; max=(pow2 32)-1});
+  mcn_encrypted_sender_data: blbytes ({min=0; max=255});
+  mcn_ciphertext: blbytes ({min=0; max=(pow2 32)-1});
+}
+
+#push-options "--ifuel 4"
+val ps_mls_ciphertext: parser_serializer mls_ciphertext_nt
+let ps_mls_ciphertext =
+  isomorphism mls_ciphertext_nt
+    (
+      _ <-- ps_bytes _;
+      _ <-- ps_u64;
+      _ <-- ps_content_type;
+      _ <-- ps_bytes _;
+      _ <-- ps_bytes _;
+      ps_bytes _
+    )
+    (fun (|group_id, (|epoch, (|content_type, (|authenticated_data, (|encrypted_sender_data, ciphertext|)|)|)|)|) -> ({
+      mcn_group_id = group_id;
+      mcn_epoch = epoch;
+      mcn_content_type = content_type;
+      mcn_authenticated_data = authenticated_data;
+      mcn_encrypted_sender_data = encrypted_sender_data;
+      mcn_ciphertext = ciphertext;
+    }))
+    (fun x -> (|x.mcn_group_id, (|x.mcn_epoch, (|x.mcn_content_type, (|x.mcn_authenticated_data, (|x.mcn_encrypted_sender_data, x.mcn_ciphertext|)|)|)|)|))
+#pop-options
+
+noeq type mls_ciphertext_content_nt (content_type: content_type_nt) = {
+  mccn_content: get_content_type content_type;
+  mccn_signature: blbytes ({min=0; max=(pow2 16)-1});
+  mccn_confirmation_tag: option_nt mac_nt;
+  mccn_padding: blbytes ({min=0; max=(pow2 16)-1});
+}
+
+val ps_mls_ciphertext_content: content_type:content_type_nt -> parser_serializer (mls_ciphertext_content_nt content_type)
+let ps_mls_ciphertext_content content_type =
+  isomorphism (mls_ciphertext_content_nt content_type)
+    (
+      _ <-- (
+        (match content_type with
+        | CT_application -> ps_bytes ({min=0; max=(pow2 32)-1})
+        | CT_proposal -> ps_proposal
+        | CT_commit -> ps_commit
+        | _ -> ps_unit
+        ) <: parser_serializer_unit (get_content_type content_type)
+      );
+      _ <-- ps_bytes _;
+      _ <-- ps_option ps_mac;
+      ps_bytes _
+    )
+    (fun (|content, (|signature, (|confirmation_tag, padding|)|)|) -> ({
+      mccn_content = content;
+      mccn_signature = signature;
+      mccn_confirmation_tag = confirmation_tag;
+      mccn_padding = padding;
+    }))
+    (fun x -> (|x.mccn_content, (|x.mccn_signature, (|x.mccn_confirmation_tag, x.mccn_padding|)|)|))
+
+noeq type mls_ciphertext_content_aad_nt = {
+  mccan_group_id: blbytes ({min=0; max=255});
+  mccan_epoch: uint64;
+  mccan_content_type: content_type_nt;
+  mccan_authenticated_data: blbytes ({min=0; max=(pow2 32)-1});
+}
+
+val ps_mls_ciphertext_content_aad: parser_serializer mls_ciphertext_content_aad_nt
+let ps_mls_ciphertext_content_aad =
+  isomorphism mls_ciphertext_content_aad_nt
+    (
+      _ <-- ps_bytes _;
+      _ <-- ps_u64;
+      _ <-- ps_content_type;
+      ps_bytes _
+    )
+    (fun (|group_id, (|epoch, (|content_type, authenticated_data|)|)|) -> ({
+      mccan_group_id = group_id;
+      mccan_epoch = epoch;
+      mccan_content_type = content_type;
+      mccan_authenticated_data = authenticated_data;
+    }))
+    (fun x -> (|x.mccan_group_id, (|x.mccan_epoch, (|x.mccan_content_type, x.mccan_authenticated_data|)|)|))
+
+noeq type mls_sender_data_nt = {
+  msdn_sender: uint32;
+  msdn_generation: uint32;
+  msdn_reuse_guard: lbytes 4;
+}
+
+val ps_mls_sender_data: parser_serializer mls_sender_data_nt
+let ps_mls_sender_data =
+  isomorphism mls_sender_data_nt
+    (
+      _ <-- ps_u32;
+      _ <-- ps_u32;
+      ps_lbytes 4
+    )
+    (fun (|sender, (|generation, reuse_guard|)|) -> ({
+      msdn_sender = sender;
+      msdn_generation = generation;
+      msdn_reuse_guard = reuse_guard;
+    }))
+    (fun x -> (|x.msdn_sender, (|x.msdn_generation, x.msdn_reuse_guard|)|))
+
+noeq type mls_sender_data_aad_nt = {
+  msdan_group_id: blbytes ({min=0; max=255});
+  msdan_epoch: uint64;
+  msdan_content_type: content_type_nt;
+}
+
+val ps_mls_sender_data_aad: parser_serializer mls_sender_data_aad_nt
+let ps_mls_sender_data_aad =
+  isomorphism mls_sender_data_aad_nt
+    (
+      _ <-- ps_bytes _;
+      _ <-- ps_u64;
+      ps_content_type
+    )
+    (fun (|group_id, (|epoch, content_type|)|) -> ({
+      msdan_group_id = group_id;
+      msdan_epoch = epoch;
+      msdan_content_type = content_type;
+    }))
+    (fun x -> (|x.msdan_group_id, (|x.msdan_epoch, x.msdan_content_type|)|))
