fstar/new/NetworkBinder.fst
@@ -1,0 +1,11 @@
+module NetworkBinder
+
+open NetworkTypes
+open Lib.Result
+
+val network_to_option: #a:Type -> option_nt a -> result (option a)
+let network_to_option #a opt =
+  match opt with
+  | None_nt -> return None
+  | Some_nt x -> return (Some x)
+  | _ -> fail "network_to_option: not a valid option"
