fstar/new/Test.Equality.fsti
@@ -1,0 +1,5 @@
+module Test.Equality
+
+open FStar.All
+
+val test_equality: #a:Type -> a -> a -> ML bool
