fstar/new/TreeDEM.Message.Content.fst
@@ -1,0 +1,131 @@
+module TreeDEM.Message.Content
+
+open Lib.ByteSequence
+open NetworkTypes
+open NetworkBinder
+open Lib.Result
+
+type message_content_type =
+  | CT_application
+  | CT_proposal
+  | CT_commit
+
+val valid_network_message_content_type: content_type_nt -> bool
+let valid_network_message_content_type content_type =
+  match content_type with
+  | NetworkTypes.CT_application -> true
+  | NetworkTypes.CT_proposal -> true
+  | NetworkTypes.CT_commit -> true
+  | _ -> false
+
+val network_to_message_content_type_tot: content_type:content_type_nt{valid_network_message_content_type content_type} -> message_content_type
+let network_to_message_content_type_tot content_type =
+  match content_type with
+  | NetworkTypes.CT_application -> CT_application
+  | NetworkTypes.CT_proposal -> CT_proposal
+  | NetworkTypes.CT_commit -> CT_commit
+
+val network_to_message_content_type: content_type_nt -> result message_content_type
+let network_to_message_content_type content_type =
+  if valid_network_message_content_type content_type then
+    return (network_to_message_content_type_tot content_type)
+  else
+    fail "network_to_message_content_type: invalid content type"
+
+val message_content_type_to_network: message_content_type -> content_type_nt
+let message_content_type_to_network content_type =
+  match content_type with
+  | CT_application -> NetworkTypes.CT_application
+  | CT_proposal -> NetworkTypes.CT_proposal
+  | CT_commit -> NetworkTypes.CT_commit
+
+noeq type proposal =
+  | Add: TreeSync.leaf_package_t -> proposal
+  | Update: TreeSync.leaf_package_t -> proposal
+  | Remove: nat -> proposal
+  | PreSharedKey: pre_shared_key_id_nt -> proposal
+  | ReInit: reinit_nt -> proposal
+  | ExternalInit: external_init_nt -> proposal
+  | AppAck: app_ack_nt -> proposal
+
+noeq type proposal_or_ref =
+  | Proposal: proposal -> proposal_or_ref
+  | Reference: bytes -> proposal_or_ref
+
+noeq type commit = {
+  c_proposals: list proposal_or_ref;
+  c_path: option (update_path_nt);
+}
+
+val message_content: message_content_type -> Type0
+let message_content content_type =
+  match content_type with
+  | CT_application -> bytes
+  | CT_proposal -> proposal
+  | CT_commit -> commit
+
+val network_to_proposal: proposal_nt -> result proposal
+let network_to_proposal p =
+  match p with
+  | P_add add ->
+    kp <-- TreeSyncTreeKEMBinder.key_package_to_treesync add.an_key_package;
+    return (Add kp)
+  | P_update update ->
+    kp <-- TreeSyncTreeKEMBinder.key_package_to_treesync update.un_key_package;
+    return (Update kp)
+  | P_remove remove ->
+    return (Remove (Lib.IntTypes.v remove.rn_removed))
+  | P_psk psk ->
+    return (PreSharedKey psk.pskn_psk)
+  | P_reinit reinit ->
+    return (ReInit reinit)
+  | P_external_init external_init ->
+    return (ExternalInit external_init)
+  | P_app_ack app_ack ->
+    return (AppAck app_ack)
+  | _ -> fail "network_to_proposal: invalid proposal"
+
+val network_to_proposal_or_ref: proposal_or_ref_nt -> result proposal_or_ref
+let network_to_proposal_or_ref por =
+  match por with
+  | POR_proposal p ->
+    res <-- network_to_proposal p;
+    return (Proposal res)
+  | POR_reference r ->
+    return (Reference r)
+  | _ -> fail "network_to_proposal_or_ref: invalid proposal or ref"
+
+val network_to_commit: commit_nt -> result commit
+let network_to_commit c =
+  proposals <-- mapM network_to_proposal_or_ref (Seq.seq_to_list c.cn_proposals);
+  path <-- network_to_option c.cn_path;
+  return ({
+    c_proposals = proposals;
+    c_path = path;
+  })
+
+val network_to_message_content: #content_type: content_type_nt{valid_network_message_content_type content_type} -> get_content_type content_type -> result (message_content (network_to_message_content_type_tot content_type))
+let network_to_message_content #content_type content =
+  match content_type with
+  | NetworkTypes.CT_application ->
+    return content
+  | NetworkTypes.CT_proposal ->
+    network_to_proposal content
+  | NetworkTypes.CT_commit ->
+    network_to_commit content
+
+let message_content_pair: Type0 = content_type:message_content_type & message_content content_type
+
+val network_to_message_content_pair: mls_content_nt -> result message_content_pair
+let network_to_message_content_pair content =
+  let make_message_content_pair (#content_type:message_content_type) (msg:message_content content_type): message_content_pair =
+    (|content_type, msg|)
+  in
+  match content with
+  | MC_application msg
+  | MC_proposal msg
+  | MC_commit msg ->
+    res <-- network_to_message_content msg;
+    return (make_message_content_pair res)
+  | _ -> fail "network_to_message_content_pair: invalid content type"
+
